tests/kind_of_term.v
@@ -1,0 +1,17 @@
+Require Import Mtac2.Base.
+Import M.
+
+(* just testing it works *)
+Definition test := ltac:(mrun (isLambda (fun x:nat=>x))).
+
+Goal eval (isLambda (fun x:nat=>x)) = true. reflexivity. Qed.
+
+Goal eval (isProd (forall x:nat, True)) = true. reflexivity. Qed.
+
+Goal eval (isCast (True : Prop)) = true. reflexivity. Qed.
+
+Goal eval (isApp (id 0)) = true. reflexivity. Qed.
+
+Goal eval (isConst (@id)) = true. reflexivity. Qed.
+
+Goal eval (isConstruct S) = true. reflexivity. Qed.
