theories/intf/Tm_kind.v
@@ -1,0 +1,15 @@
+Inductive tm_kind :=
+  | tmVar
+  | tmEvar
+  | tmSort
+  | tmConst
+  | tmConstruct
+  | tmProd
+  | tmLambda
+  | tmLetIn
+  | tmApp
+  | tmCast
+  | tmInd
+  | tmCase
+  | tmFix
+  | tmCoFix.
